common.v
@@ -1,0 +1,2 @@
+From PER Require Export syntax.
+Definition context n := fin n -> ty.
